Sal/MRDTs/Metatheory/NegativeLedger.lean
@@ -8,6 +8,7 @@ import Sal.MRDTs.Instances.AegisSheetMaterialisedCertificates
 import Sal.MRDTs.Instances.AegisSheetMaterialisedEquivalence
 import Sal.MRDTs.Instances.AegisSheetMaterialisedUpdate
 import Sal.MRDTs.Instances.AegisSheetMaterialisedBridge
+import Sal.MRDTs.Instances.AegisSheetMaterialisedConverse
 import Sal.MRDTs.Instances.FugueMaxReplay
 import Sal.MRDTs.Metatheory.ConditioningSPOT
 import Sal.MRDTs.Metatheory.Join.Convergence_CounterModel
@@ -54,6 +55,8 @@ namespace Sal.MRDTs.Negative
 #check Instances.AegisSheet.Materialised.verified
 #check Instances.AegisSheet.Materialised.issued_of_version
 #check Instances.AegisSheet.Materialised.cross_model
+#check Instances.AegisSheet.Materialised.UndoHonest
+#check Instances.AegisSheet.Materialised.converse
 #check Instances.SidedEmbedRGA.fmGeneration
 #check Instances.SidedEmbedRGA.fmReplayAdequacy
 #check Instances.SidedEmbedRGA.fuguemax_replay_witness
